rustfrontend/RustIRown.v
@@ -744,7 +744,7 @@ evaluated to pointer as it is ill-formed. *)
     (* The reason we do not support p2 to be downcast is written in
     the proof of the absence of step_assign_variant_error6 in
     MoveCheckingSafe.v *)
-    (NODOWN: forall ty fid, ~ In (ph_downcast ty fid) (snd (path_of_place p2)))
+    (NODOWN: forall  fid, ~ In (proj_downcast fid) (snd (path_of_place p2)))
     (EVALE: eval_place ge le m1 p2 b2 ofs2)
     (COPYTY: access_mode ty = By_copy)
     (* we do not support ZST for now *)
