Makefile
@@ -172,12 +172,12 @@ RUSTFRONTEND=Rusttypes.v Rustsyntax.v Rustlight.v RustIR.v\
   Rustlightgen.v\
   RustIRgen.v RustIRgenProof.v RustIRcfg.v\
   InitDomain.v InitAnalysis.v ElaborateDrop.v ElaborateDropProof.v\
-  MoveChecking.v MoveCheckingFootprint.v MoveCheckingFootprint1.v MoveCheckingDomain.v \
+  MoveChecking.v MoveCheckingFootprint1.v \
   Clightgen.v Clightgenspec.v Clightgenproof.v\
   RustOp.v Rusttyping.v\
   StkBorPermission.v RustIRbor.v\
   BorrowCheckDomain.v ReplaceOrigins.v BorrowCheckPolonius.v\
-  RegionLiveness.v BorrowCheck.v BorrowCheckSound.v\
+  RegionLiveness.v BorrowCheck.v \
   Listmisc.v\
   # BorrowCheckSafe.v
 
